Add draft for proof of crash_impl_sat

TransVal/Crash.v
@@ -2,7 +2,7 @@ Require Import IL StateType.
 
 Inductive Crash : F.state -> F.state -> Prop :=
 |CrashBase L E s :
- (forall a σ, ~ F.step (L, E, s) a σ)
+ normal2 F.step (L, E, s)
 -> state_result (L,E,s) = None
 -> Crash (L, E,s) (L,E,s)
 |CrashStep sigma sigma' sigma'' a:
